SmallStepSemantics.v
@@ -1,6 +1,7 @@
 Require Import Coq.Lists.List.
 Require Import PL.Imp3.
 Require Import PL.ImpExt4.
+Require Import PL.DenotationalSemantics.
 
 Require Import Coq.Classes.Morphisms.
 Require Import Coq.Classes.Morphisms_Prop.
@@ -113,20 +114,6 @@ Proof.
     - apply IHclos_refl_trans_1n, H1.
 Qed.
 
-Lemma rt1n_trans_again: forall A (R: A -> A -> Prop) a b c,
-  clos_refl_trans_1n R a b ->
-  clos_refl_trans_1n R b c ->
-  clos_refl_trans_1n R a c.
-Proof.
-  intros.
-  induction H.
-  + exact H0.
-  + apply IHclos_refl_trans_1n in H0.
-    apply rt1n_trans_1n with y.
-    - exact H.
-    - exact H0.
-Qed.
-
 Lemma rtn1_trans: forall A (R: A -> A -> Prop) a b c,
   clos_refl_trans_n1 R a b ->
   clos_refl_trans_n1 R b c ->
@@ -203,6 +190,8 @@ Proof.
   hnf; intros.
   eapply rt_trans; eauto.
 Qed.
+
+
 Lemma ind_1N: forall A (R RT_R: A -> A -> Prop),
   (RT_R = clos_refl_trans R) ->
   forall x (P: A -> Prop),
@@ -400,36 +389,720 @@ Inductive cstep : (com * state) -> bool -> (com * state) -> Prop :=
         false
         ((If b Then (c;; While b Do c EndWhile) Else Skip EndIf)%imp, st).
 
-Inductive clos_refl_trans {A B : Type} (base : A -> bool -> A -> B)
-                                       (add : B -> B -> B)
+Inductive clos_refl_trans {A B : Type} (mp : mid_param A B)
                                        (R : A -> bool -> A -> Prop)
                                        : A -> B -> A -> Prop :=
-    rt_step : forall x y b, R x b y -> clos_refl_trans base add R x (base x b y) y
-  | rt_refl : forall x, clos_refl_trans base add R x (base x false x) x
+    rt_step_false : forall x y, R x false y -> clos_refl_trans mp R x (MP_zero mp) y
+  | rt_step_true : forall x y, R x true y -> clos_refl_trans mp R x (MP_one mp x y) y
+  | rt_refl : forall x, clos_refl_trans mp R x (MP_zero mp) x
   | rt_trans : forall x y z c1 c2,
-               clos_refl_trans base add R x c1 y ->
-               clos_refl_trans base add R y c2 z -> clos_refl_trans base add R x (add c1 c2) z.
+               clos_refl_trans mp R x c1 y ->
+               clos_refl_trans mp R y c2 z ->
+               clos_refl_trans mp R x (MP_add mp c1 c2) z.
 
-Definition base_cnt (_ : com * state) (b : bool) (_ : com * state) : Z :=
-  match b with
-  | false => 0
-  | true => 1
-  end.
+Inductive clos_refl_trans_1n {A B : Type} (mp : mid_param A B)
+                                          (R : A -> bool -> A -> Prop)
+                                          : A -> B -> A -> Prop :=
+    | rt1n_refl : forall x, clos_refl_trans_1n mp R x (MP_zero mp) x
+    | rt1n_trans_1n_false : forall x y z c,
+          R x false y ->
+          clos_refl_trans_1n mp R y c z ->
+          clos_refl_trans_1n mp R x c z
+    | rt1n_trans_1n_true : forall x y z c,
+          R x true y ->
+          clos_refl_trans_1n mp R y c z ->
+          clos_refl_trans_1n mp R x (MP_add mp (MP_one mp x y) c) z.
 
-Definition multi_cstep_cnt: com * state -> Z -> com * state -> Prop := 
-  clos_refl_trans base_cnt Z.add cstep.
+Inductive clos_refl_trans_n1 {A B : Type} (mp : mid_param A B)
+                                          (R : A -> bool -> A -> Prop)
+                                          : A -> B -> A -> Prop :=
+    | rtn1_refl : forall x, clos_refl_trans_n1 mp R x (MP_zero mp) x
+    | rtn1_trans_n1_false : forall x y z c,
+          R y false z ->
+          clos_refl_trans_n1 mp R x c y ->
+          clos_refl_trans_n1 mp R x c z
+    | rtn1_trans_n1_true : forall x y z c,
+          R y true z ->
+          clos_refl_trans_n1 mp R x c y ->
+          clos_refl_trans_n1 mp R x (MP_add mp c (MP_one mp y z)) z.
 
-Definition base_trace (_ : com * state) (b : bool) (cst : com * state) : list state :=
-  match b with
-  | false => nil
-  | true => match cst with
-    | (c, st) => (st :: nil)
+Lemma rt_trans_1n_false: forall A B (mp : mid_param A B) (R: A -> bool -> A -> Prop) x y z c,
+  R x false y ->
+  clos_refl_trans mp R y c z ->
+  clos_refl_trans mp R x c z.
+Proof.
+  intros.
+  rewrite <- (MP_add_zero_l mp c).
+  eapply rt_trans with y; [| exact H0].
+  apply rt_step_false.
+  exact H.
+Qed.
+
+Lemma rt_trans_1n_true: forall A B (mp : mid_param A B) (R: A -> bool -> A -> Prop) x y z c,
+  R x true y ->
+  clos_refl_trans mp R y c z ->
+  clos_refl_trans mp R x (MP_add mp (MP_one mp x y) c) z.
+Proof.
+  intros.
+  eapply rt_trans with y; [| exact H0].
+  apply rt_step_true.
+  exact H.
+Qed.
+
+Lemma rt_trans_n1_false: forall A B (mp : mid_param A B) (R: A -> bool -> A -> Prop) x y z c,
+  R y false z ->
+  clos_refl_trans mp R x c y ->
+  clos_refl_trans mp R x c z.
+Proof.
+  intros.
+  rewrite <- (MP_add_zero_r mp c).
+  eapply rt_trans with y; [exact H0 |].
+  apply rt_step_false.
+  exact H.
+Qed.
+
+Lemma rt_trans_n1_true: forall A B (mp : mid_param A B) (R: A -> bool -> A -> Prop) x y z c,
+  R y true z ->
+  clos_refl_trans mp R x c y ->
+  clos_refl_trans mp R x (MP_add mp c (MP_one mp y z)) z.
+Proof.
+  intros.
+  eapply rt_trans with y; [exact H0 |].
+  apply rt_step_true.
+  exact H.
+Qed.
+
+Lemma rt1n_step_false: forall A B (mp : mid_param A B) (R: A -> bool -> A -> Prop) x y,
+  R x false y ->
+  clos_refl_trans_1n mp R x (MP_zero mp) y.
+Proof.
+  intros.
+  apply rt1n_trans_1n_false with y.
+  + exact H.
+  + apply rt1n_refl.
+Qed.
+
+Lemma rt1n_step_true: forall A B (mp : mid_param A B) (R: A -> bool -> A -> Prop) x y,
+  R x true y ->
+  clos_refl_trans_1n mp R x (MP_one mp x y) y.
+Proof.
+  intros.
+  rewrite <- (MP_add_zero_r mp _).
+  apply rt1n_trans_1n_true.
+  + exact H.
+  + apply rt1n_refl.
+Qed.
+
+Lemma rtn1_step_false: forall A B (mp : mid_param A B) (R: A -> bool -> A -> Prop) x y,
+  R x false y ->
+  clos_refl_trans_n1 mp R x (MP_zero mp) y.
+Proof.
+  intros.
+  apply rtn1_trans_n1_false with x.
+  + exact H.
+  + apply rtn1_refl.
+Qed.
+
+Lemma rtn1_step_true: forall A B (mp : mid_param A B) (R: A -> bool -> A -> Prop) x y,
+  R x true y ->
+  clos_refl_trans_n1 mp R x (MP_one mp x y) y.
+Proof.
+  intros.
+  rewrite <- (MP_add_zero_l mp _).
+  apply rtn1_trans_n1_true.
+  + exact H.
+  + apply rtn1_refl.
+Qed.
+
+Lemma rt1n_trans: forall A B (mp : mid_param A B) (R: A -> bool -> A -> Prop) x y z c1 c2,
+  clos_refl_trans_1n mp R x c1 y ->
+  clos_refl_trans_1n mp R y c2 z ->
+  clos_refl_trans_1n mp R x (MP_add mp c1 c2) z.
+Proof.
+  intros.
+  revert H0.
+  induction H; intros.
+  + rewrite -> (MP_add_zero_l mp). tauto.
+  + apply rt1n_trans_1n_false with y.
+    - exact H.
+    - apply IHclos_refl_trans_1n, H1.
+  + rewrite -> (MP_add_assoc mp).
+    apply rt1n_trans_1n_true.
+    - exact H.
+    - apply IHclos_refl_trans_1n, H1.
+Qed.
+
+Lemma rtn1_trans: forall A B (mp : mid_param A B) (R: A -> bool -> A -> Prop) x y z c1 c2,
+  clos_refl_trans_n1 mp R x c1 y ->
+  clos_refl_trans_n1 mp R y c2 z ->
+  clos_refl_trans_n1 mp R x (MP_add mp c1 c2) z.
+Proof.
+  intros.
+  induction H0.
+  + rewrite -> (MP_add_zero_r mp). tauto.
+  + apply rtn1_trans_n1_false with y; tauto.
+  + rewrite <- (MP_add_assoc mp).
+    apply rtn1_trans_n1_true; tauto.
+Qed.
+
+Lemma rt1n_rt: forall A B (mp : mid_param A B) (R: A -> bool -> A -> Prop) x y c,
+  clos_refl_trans_1n mp R x c y -> clos_refl_trans mp R x c y.
+Proof.
+  intros.
+  induction H.
+  + apply rt_refl.
+  + apply rt_trans_1n_false with y; tauto.
+  + apply rt_trans_1n_true; tauto.
+Qed.
+
+Lemma rt_rt1n: forall A B (mp : mid_param A B) (R: A -> bool -> A -> Prop) x y c,
+  clos_refl_trans mp R x c y -> clos_refl_trans_1n mp R x c y.
+Proof.
+  intros.
+  induction H.
+  + apply rt1n_step_false, H.
+  + apply rt1n_step_true, H.
+  + apply rt1n_refl.
+  + apply rt1n_trans with y; tauto.
+Qed.
+
+Lemma rtn1_rt: forall A B (mp : mid_param A B) (R: A -> bool -> A -> Prop) x y c,
+  clos_refl_trans_n1 mp R x c y -> clos_refl_trans mp R x c y.
+Proof.
+  intros.
+  induction H.
+  + apply rt_refl.
+  + apply rt_trans_n1_false with y; tauto.
+  + apply rt_trans_n1_true; tauto.
+Qed.
+
+Lemma rt_rtn1: forall A B (mp : mid_param A B) (R: A -> bool -> A -> Prop) x y c,
+  clos_refl_trans mp R x c y -> clos_refl_trans_n1 mp R x c y.
+Proof.
+  intros.
+  induction H.
+  + apply rtn1_step_false, H.
+  + apply rtn1_step_true, H.
+  + apply rtn1_refl.
+  + apply rtn1_trans with y; tauto.
+Qed.
+
+Lemma rt_rt1n_iff: forall A B (mp : mid_param A B) (R: A -> bool -> A -> Prop) x y c,
+  clos_refl_trans mp R x c y <-> clos_refl_trans_1n mp R x c y.
+Proof.
+  split; intros.
+  + apply rt_rt1n; auto.
+  + apply rt1n_rt; auto.
+Qed.
+
+Lemma rt_rtn1_iff: forall A B (mp : mid_param A B) (R: A -> bool -> A -> Prop) x y c,
+  clos_refl_trans mp R x c y <-> clos_refl_trans_n1 mp R x c y.
+Proof.
+  split; intros.
+  + apply rt_rtn1; auto.
+  + apply rtn1_rt; auto.
+Qed.
+
+Lemma rt_refl_zero: forall A B (mp : mid_param A B) (R: A -> bool -> A -> Prop) (RT_R: A -> B -> A -> Prop),
+  (RT_R = clos_refl_trans mp R) ->
+  forall x c,
+  (c = MP_zero mp) -> clos_refl_trans mp R x c x.
+Proof. intros. subst. apply rt_refl. Qed.
+
+Lemma rt_trans_add: forall A B (mp : mid_param A B) (R: A -> bool -> A -> Prop) (RT_R: A -> B -> A -> Prop),
+  (RT_R = clos_refl_trans mp R) ->
+  forall x y z c1 c2 c3,
+    RT_R x c1 y ->
+    c3 = MP_add mp c1 c2 ->
+    RT_R y c2 z ->
+    RT_R x c3 z.
+Proof. intros. subst. apply rt_trans with y; tauto. Qed.
+
+Lemma ind_1N: forall A B (mp : mid_param A B) (R: A -> bool -> A -> Prop) (RT_R: A -> B -> A -> Prop),
+  (RT_R = clos_refl_trans mp R) ->
+  forall x (P: A -> B -> Prop),
+  P x (MP_zero mp) ->
+  (forall y z c (IH: P y c), R z false y -> RT_R y c x -> P z c) ->
+  (forall y z c (IH: P y c), R z true y -> RT_R y c x -> P z (MP_add mp (MP_one mp z y) c)) ->
+  (forall y c, RT_R y c x -> P y c).
+Proof.
+  intros.
+  subst RT_R.
+  apply rt_rt1n in H3.
+  induction H3; auto.
+  apply H1 with y; auto.
+  apply rt1n_rt; auto.
+  apply H2; auto.
+  apply rt1n_rt; auto.
+Qed.
+
+Lemma ind_N1: forall A B (mp : mid_param A B) (R: A -> bool -> A -> Prop) (RT_R: A -> B -> A -> Prop),
+  (RT_R = clos_refl_trans mp R) ->
+  forall x (P: A -> B -> Prop),
+  P x (MP_zero mp) ->
+  (forall y z c (IH: P y c), R y false z -> RT_R x c y -> P z c) ->
+  (forall y z c (IH: P y c), R y true z -> RT_R x c y -> P z (MP_add mp c (MP_one mp y z))) ->
+  (forall y c, RT_R x c y -> P y c).
+Proof.
+  intros.
+  subst RT_R.
+  apply rt_rtn1 in H3.
+  induction H3; auto.
+  apply H1 with y; auto.
+  apply rtn1_rt; auto.
+  apply H2; auto.
+  apply rtn1_rt; auto.
+Qed.
+
+Lemma trans_1N_false: forall A B (mp : mid_param A B) (R: A -> bool -> A -> Prop) (RT_R: A -> B -> A -> Prop),
+  (RT_R = clos_refl_trans mp R) ->
+  forall x y z c, R x false y -> RT_R y c z -> RT_R x c z.
+Proof.
+  intros.
+  subst.
+  apply rt_trans_1n_false with y; auto.
+Qed.
+
+Lemma trans_1N_true: forall A B (mp : mid_param A B) (R: A -> bool -> A -> Prop) (RT_R: A -> B -> A -> Prop),
+  (RT_R = clos_refl_trans mp R) ->
+  forall x y z c c', R x true y -> RT_R y c z -> (c' = MP_add mp (MP_one mp x y) c) -> RT_R x c' z.
+Proof.
+  intros.
+  subst.
+  apply rt_trans_1n_true; auto.
+Qed.
+
+Lemma trans_1N: forall A B (mp : mid_param A B) (R: A -> bool -> A -> Prop) (RT_R: A -> B -> A -> Prop),
+  (RT_R = clos_refl_trans mp R) ->
+  forall x y z c b c', R x b y ->
+    (if b then c' = (MP_add mp (MP_one mp x y) c) else c' = c) ->
+    RT_R y c z ->
+    RT_R x c' z.
+Proof.
+  intros.
+  destruct b; inversion H1; subst.
+  apply (trans_1N_true _ _ _ R _ eq_refl x y z c _ H0 H2 eq_refl).
+  apply (trans_1N_false _ _ _ R _ eq_refl x y z c H0 H2).
+Qed.
+
+Lemma trans_N1_false: forall A B (mp : mid_param A B) (R: A -> bool -> A -> Prop) (RT_R: A -> B -> A -> Prop),
+  (RT_R = clos_refl_trans mp R) ->
+  forall x y z c, RT_R x c y -> R y false z -> RT_R x c z.
+Proof.
+  intros.
+  subst.
+  apply rt_trans_n1_false with y; auto.
+Qed.
+
+Lemma trans_N1_true: forall A B (mp : mid_param A B) (R: A -> bool -> A -> Prop) (RT_R: A -> B -> A -> Prop),
+  (RT_R = clos_refl_trans mp R) ->
+  forall x y z c c', RT_R x c y -> R y true z -> c' = MP_add mp c (MP_one mp y z) -> RT_R x c' z.
+Proof.
+  intros.
+  subst.
+  apply rt_trans_n1_true; auto.
+Qed.
+
+Lemma trans_N1: forall A B (mp : mid_param A B) (R: A -> bool -> A -> Prop) (RT_R: A -> B -> A -> Prop),
+  (RT_R = clos_refl_trans mp R) ->
+  forall x y z c (b: bool) c', RT_R x c y ->
+    (if b then c' = (MP_add mp c (MP_one mp y z)) else c' = c) ->
+    R y b z ->
+    RT_R x c' z.
+Proof.
+  intros.
+  destruct b; inversion H1; subst.
+  apply (trans_N1_true _ _ _ R _ eq_refl x y z c _ H0 H2 eq_refl).
+  apply (trans_N1_false _ _ _ R _ eq_refl x y z c H0 H2).
+Qed.
+
+Ltac induction_1n H :=
+  match type of H with
+  | ?RT_R ?b ?c ?a =>
+    revert_dependent_component b H;
+    let b0 := fresh "b" in
+    let c0 := fresh "c" in
+    let EQb := fresh "EQb" in
+    let EQc := fresh "EQc" in
+    remember b as b0 eqn:EQb in H;
+    remember c as c0 eqn:EQc in H;
+    revert EQb EQc;
+    revert_component b;
+    revert_component c;
+    match goal with
+    | |- ?Q =>
+      let Pbc := eval pattern c0 in Q in
+      match Pbc with
+      | ?Q' c0 =>
+        let Pb := eval pattern b0 in Q' in
+        match Pb with
+        | ?P b0 =>
+          revert b0 c0 H;
+          refine (ind_1N _ _ _ _ RT_R eq_refl a P _ _ _);
+          [ first [rewrite (MP_MP_zero _ _ _ _ _ _ _ eq_refl)| idtac];
+            intros_until_EQ EQb;
+            intros_until_EQ EQc;
+            match goal with
+            | |- ?Base =>
+              let Base0 := fresh in
+              remember Base as Base0 in |- *;
+              first [ injection EQb; clear EQb; intros_and_subst Base0
+                    | revert EQb; intros_and_subst Base0
+                    | subst b0
+                    | idtac ];
+              subst Base0
+            end;
+            match goal with
+            | |- ?Base =>
+              let Base0 := fresh in
+              remember Base as Base0 in |- *;
+              first [ injection EQc; clear EQc; intros_and_subst Base0
+                    | revert EQc; intros_and_subst Base0
+                    | subst c0
+                    | idtac ];
+              subst Base0
+            end
+          | let b0 := fresh "x" in
+            let c0 := fresh "c" in
+            let H0 := fresh "H" in
+            let IH := fresh "IHrt" in
+            first [intros ?b b0 c0 IH H0 ? | intros ? b0 c0 IH H0 ?];
+            intros_until_EQ EQb;
+            intros_until_EQ EQc;
+            subst b0;
+            repeat progress
+            match type of H0 with
+            | _ ?y ?c ?x => destruct_to_form x y
+            end;
+            specialize_until_EQ IH;
+            specialize_until_EQ IH
+          | first [ rewrite (MP_MP_one _ _ _ _ _ _ _ eq_refl);
+                    rewrite (MP_MP_add _ _ _ _ _ _ _ eq_refl)
+                  | idtac];
+            let b0 := fresh "x" in
+            let c0 := fresh "c" in
+            let H0 := fresh "H" in
+            let IH := fresh "IHrt" in
+            first [intros ?b b0 c0 IH H0 ? | intros ? b0 c0 IH H0 ?];
+            intros_until_EQ EQb;
+            intros_until_EQ EQc;
+            subst b0;
+            repeat progress
+            match type of H0 with
+            | _ ?y ?c ?x => destruct_to_form x y
+            end;
+            specialize_until_EQ IH;
+            specialize_until_EQ IH
+          ]
+        end
+      end
     end
   end.
 
+Ltac induction_n1 H :=
+  match type of H with
+  | ?RT_R ?a ?c ?b =>
+    revert_dependent_component b H;
+    let b0 := fresh "b" in
+    let c0 := fresh "c" in
+    let EQb := fresh "EQb" in
+    let EQc := fresh "EQc" in
+    remember b as b0 eqn:EQb in H;
+    remember c as c0 eqn:EQc in H;
+    revert EQb EQc;
+    revert_component b;
+    revert_component c;
+    match goal with
+    | |- ?Q =>
+      let Pbc := eval pattern c0 in Q in
+      match Pbc with
+      | ?Q' c0 =>
+        let Pb := eval pattern b0 in Q' in
+        match Pb with
+        | ?P b0 =>
+          revert b0 c0 H;
+          refine (ind_N1 _ _ _ _ RT_R eq_refl a P _ _ _);
+          [ first [rewrite (MP_MP_zero _ _ _ _ _ _ _ eq_refl)| idtac];
+            intros_until_EQ EQb;
+            intros_until_EQ EQc;
+            match goal with
+            | |- ?Base =>
+              let Base0 := fresh in
+              remember Base as Base0 in |- *;
+              first [ injection EQb; clear EQb; intros_and_subst Base0
+                    | revert EQb; intros_and_subst Base0
+                    | subst b0
+                    | idtac ];
+              subst Base0
+            end;
+            match goal with
+            | |- ?Base =>
+              let Base0 := fresh in
+              remember Base as Base0 in |- *;
+              first [ injection EQc; clear EQc; intros_and_subst Base0
+                    | revert EQc; intros_and_subst Base0
+                    | subst c0
+                    | idtac ];
+              subst Base0
+            end
+          | let b0 := fresh "x" in
+            let c0 := fresh "c" in
+            let H0 := fresh "H" in
+            let IH := fresh "IHrt" in
+            first [intros ?b b0 c0 IH H0 ? | intros ? b0 c0 IH H0 ?];
+            intros_until_EQ EQb;
+            intros_until_EQ EQc;
+            subst b0;
+            subst c0;
+            repeat progress
+            match type of H0 with
+            | _ ?x ?c ?y => destruct_to_form x y
+            end;
+            specialize_until_EQ IH;
+            specialize_until_EQ IH
+          | first [ rewrite (MP_MP_one _ _ _ _ _ _ _ eq_refl);
+                    rewrite (MP_MP_add _ _ _ _ _ _ _ eq_refl)
+                  | idtac];
+            let b0 := fresh "x" in
+            let c0 := fresh "c" in
+            let H0 := fresh "H" in
+            let IH := fresh "IHrt" in
+            first [intros ?b b0 c0 IH H0 ? | intros ? b0 c0 IH H0 ?];
+            intros_until_EQ EQb;
+            intros_until_EQ EQc;
+            subst b0;
+            repeat progress
+            match type of H0 with
+            | _ ?x ?c ?y => destruct_to_form x y
+            end;
+            specialize_until_EQ IH;
+            specialize_until_EQ IH
+          ]
+        end
+      end
+    end
+  end.
+
+Ltac transitivity_1n_false y :=
+  match goal with
+  | |- ?RT_R ?x ?c ?z =>
+    refine (trans_1N_false _ _ _ _ RT_R eq_refl x y z c _ _)
+  end.
+
+Ltac transitivity_1n_true y c :=
+  match goal with
+  | |- ?RT_R ?x ?c' ?z =>
+    first [ refine (trans_1N_true _ _ _ _ RT_R eq_refl x y z c c' _ _ eq_refl)
+          | refine (trans_1N_true _ _ _ _ RT_R eq_refl x y z c c' _ _ _)]
+  end.
+
+Ltac etransitivity_1n :=
+  match goal with
+  | |- ?RT_R ?x ?c ?z =>
+    match type of x with
+    | ?A =>
+      match type of c with
+      | ?B => let y := fresh "y" in
+              let b := fresh "b" in
+              let c' := fresh "c'" in
+              evar (y: A);
+              evar (b: bool);
+              evar (c': B);
+              refine (trans_1N _ _ _ _ RT_R eq_refl x y z c' b c _ _ _);
+              [ | first [ rewrite (MP_MP_one _ _ _ _ _ _ _ eq_refl);
+                          rewrite (MP_MP_add _ _ _ _ _ _ _ eq_refl)
+                        | idtac] | ];
+              subst y b c'
+      end
+    end
+  end.
+
+Ltac transitivity_n1_false y :=
+  match goal with
+  | |- ?RT_R ?x ?c ?z =>
+    refine (trans_N1_false _ _ _ _ RT_R eq_refl x y z c _ _)
+  end.
+
+Ltac transitivity_n1_true y c :=
+  match goal with
+  | |- ?RT_R ?x ?c' ?z =>
+    first [ refine (trans_N1_true _ _ _ _ RT_R eq_refl x y z c c' _ _ eq_refl)
+          | refine (trans_N1_true _ _ _ _ RT_R eq_refl x y z c c' _ _ _)]
+  end.
+
+Ltac etransitivity_n1 :=
+  match goal with
+  | |- ?RT_R ?x ?c ?z =>
+    match type of x with
+    | ?A =>
+      match type of c with
+      | ?B => let y := fresh "y" in
+              let b := fresh "b" in
+              let c' := fresh "c'" in
+              evar (y: A);
+              evar (b: bool);
+              evar (c': B);
+              refine (trans_N1 _ _ _ _ RT_R eq_refl x y z c' b c _ _ _);
+              [ | first [ rewrite (MP_MP_one _ _ _ _ _ _ _ eq_refl);
+                          rewrite (MP_MP_add _ _ _ _ _ _ _ eq_refl)
+                        | idtac] | ];
+              subst y b c'
+      end
+    end
+  end.
+
+Ltac rt_reflexivity :=
+  match goal with
+  | |- ?RT_R ?x ?c ?y =>
+    refine (rt_refl_zero _ _ _ _ RT_R eq_refl x c eq_refl)
+  end.
+
+Ltac rt_transitivity y c1 c2 :=
+  match goal with
+  | |- ?RT_R ?x ?c ?z =>
+    first [ refine (rt_trans_add _ _ _ _ RT_R eq_refl x y z c1 c2 c _ eq_refl _)
+          | refine (rt_trans_add _ _ _ _ RT_R eq_refl x y z c1 c2 c _ _ _)]
+  end.
+
+Ltac rt_etransitivity :=
+  match goal with
+  | |- ?RT_R ?x ?c ?z =>
+    match type of x with
+    | ?A =>
+      match type of c with
+      | ?B => let y := fresh "y" in
+              let c1 := fresh "c1" in
+              let c2 := fresh "c2" in
+              evar (y: A);
+              evar (c1: B);
+              evar (c2: B);
+              refine (rt_trans_add _ _ _ _ RT_R eq_refl x y z c1 c2 c _ _ _);
+              [ | first [ rewrite (MP_MP_add _ _ _ _ _ _ _ eq_refl)
+                        | idtac] | ];
+              subst y c1 c2
+      end
+    end
+  end.
+
+Definition extend_one {A B: Type} (one: A -> A -> B) (C: Type) : (C*A) -> (C*A) -> B
+:= fun ca1 ca2 =>
+     match ca1,ca2 with
+     | (c1,a1),(c2,a2) => one a1 a2
+     end.
+
+(* Lemma extend_one_preserve : forall {A B: Type} (one: A -> A -> B) (C: Type) a1 a2 c1 c2,
+  one a1 a2 =
+  (extend_one one C) (c1,a1) (c2,a2).
+Proof. intros. reflexivity. Qed. *)
+
+Definition extend_mp {A B: Type} (mp: mid_param A B) (C: Type) : mid_param (C*A) B
+:= match mp with
+   | MP zero one add add_zero_l add_zero_r add_assoc => 
+     MP zero (extend_one one C) add add_zero_l add_zero_r add_assoc
+   end.
+
+Definition multi_cstep {T: Type} (mp: mid_param state T): com * state -> T -> com * state -> Prop := 
+  clos_refl_trans (extend_mp mp com) cstep.
+
+Definition multi_cstep_cnt: com * state -> Z -> com * state -> Prop := 
+  multi_cstep Z_mp.
+
 Definition multi_cstep_trace: com * state -> list state -> com * state -> Prop :=
-  clos_refl_trans base_trace (@List.app state) cstep.
+  multi_cstep List_mp.
+
+Module TestRT.
+
+Definition test_one (_ : Z * Z) (_ : Z * Z) : Z :=
+  1.
+
+Inductive test_step : (Z * Z) -> bool -> (Z * Z) -> Prop :=
+  | TS_0 : forall a b1 b2, test_step (a, b1) false (a, b2)
+  | TS_1 : forall a b, test_step (a, b) true (a + 1, b).
+
+Definition multi_test_step: (Z * Z) -> Z -> (Z * Z) -> Prop := 
+  clos_refl_trans (MP 0 test_one Z.add Z.add_0_l Z.add_0_r Zplus_assoc_reverse) test_step.
+
+Example test_step_example: multi_test_step (1,2) 3 (4,5).
+Proof.
+  intros. rt_transitivity (2, 10) 1 2.
+  { etransitivity_1n.
+    + apply TS_0.
+    + simpl. reflexivity.
+    + etransitivity_1n.
+      * apply TS_1.
+      * unfold test_one. instantiate (c':=0). reflexivity.
+      * rt_reflexivity. }
+  rt_etransitivity.
+  { etransitivity_n1.
+    + etransitivity_n1.
+      * rt_reflexivity.
+      * unfold test_one. simpl. instantiate (b0:=false). reflexivity.
+      * apply TS_0.
+    + unfold test_one. simpl. instantiate (b:=true). reflexivity.
+    + apply TS_1. }
+  { instantiate (c2:=1). reflexivity. }
+  transitivity_1n_false (3,6).
+  { instantiate (1:=0). apply TS_0. }
+  transitivity_1n_true (4,6) 0.
+  { apply TS_1. }
+  transitivity_n1_false (4,6).
+  { rt_reflexivity. }
+  apply TS_0.
+Qed.
+
+Example test_step_equiv_minus_n1: forall a1 b1 a2 b2 c, multi_test_step (a1,b1) c (a2,b2) -> a2-a1=c.
+Proof.
+  intros.
+  remember (a1,b1) as ab1.
+  remember (a2,b2) as ab2.
+  revert Heqab1 Heqab2.
+  revert a1 b1 a2 b2.
+  induction_n1 H; intros; subst.
+  - inversion Heqab2. lia.
+  - inversion H; subst.
+    repeat specialize_until_EQ IHrt.
+    lia.
+  - inversion H; subst.
+    unfold test_one.
+    repeat specialize_until_EQ IHrt.
+    lia.
+Qed.
+
+Example test_step_equiv_minus_1n: forall a1 b1 a2 b2 c, multi_test_step (a1,b1) c (a2,b2) -> a2-a1=c.
+Proof.
+  intros.
+  remember (a1,b1) as ab1.
+  remember (a2,b2) as ab2.
+  revert Heqab1 Heqab2.
+  revert a1 b1 a2 b2.
+  induction_1n H; intros; subst.
+  - inversion Heqab2. lia.
+  - inversion H; subst.
+    repeat specialize_until_EQ IHrt.
+    lia.
+  - inversion H; subst.
+    unfold test_one.
+    repeat specialize_until_EQ IHrt.
+    lia.
+Qed.
+
+Example test_step_equiv_minus: forall a1 b1 a2 b2 c, multi_test_step (a1,b1) c (a2,b2) -> a2-a1=c.
+Proof.
+  intros.
+  remember (a1,b1) as ab1.
+  remember (a2,b2) as ab2.
+  revert Heqab1 Heqab2.
+  revert a1 b1 a2 b2.
+  induction H; intros; simpl; subst.
+  - inversion H. subst. lia.
+  - inversion H. subst. unfold test_one. lia.
+  - inversion Heqab2. lia.
+  - destruct y.
+    repeat specialize_until_EQ IHclos_refl_trans1.
+    repeat specialize_until_EQ IHclos_refl_trans2.
+    lia.
+Qed.
+
+End TestRT.
 
 End TerStep.
-
-
