DenotationalSemEquiv.v
@@ -63,47 +63,53 @@ Definition Bin_Ter_loop_sem_equiv {M: Type}
     (semantic_loop SBin b (ceval_by_sem SBin c))
     (semantic_loop STer b (ceval_by_sem STer c)).
 
-Theorem Bin_Step_skip_sem_equiv:
-  Bin_Ter_skip_sem_equiv (BinRel.sem) (StepCnt.sem).
+Theorem Bin_Ter_skip_sem_equiv_true:
+  forall {T: Type} (mp: mid_param state T),
+  Bin_Ter_skip_sem_equiv (BinRel.sem) (TerSem.sem mp).
 Proof.
+  intros.
   unfold Bin_Ter_skip_sem_equiv. simpl.
   unfold Bin_Ter_sem_equiv. intros.
-  unfold BinRel.skip_sem, StepCnt.skip_sem.
+  unfold BinRel.skip_sem, TerSem.skip_sem.
   split.
-  - intros. exists 0. tauto.
+  - intros. exists (MP_zero mp). tauto.
   - intros [z [H1 H2]].
     tauto.
 Qed.
 
-Theorem Bin_Step_asgn_sem_equiv:
-  Bin_Ter_asgn_sem_equiv (BinRel.sem) (StepCnt.sem).
+Theorem Bin_Ter_asgn_sem_equiv_true:
+  forall {T: Type} (mp: mid_param state T),
+  Bin_Ter_asgn_sem_equiv (BinRel.sem) (TerSem.sem mp).
 Proof.
+  intros.
   unfold Bin_Ter_asgn_sem_equiv. simpl.
   unfold Bin_Ter_sem_equiv. intros.
-  unfold BinRel.asgn_sem,StepCnt.asgn_sem.
+  unfold BinRel.asgn_sem,TerSem.asgn_sem.
   split.
-  - intros [H1 H2]. exists 1.
+  - intros [H1 H2]. exists (MP_one mp st1 st2).
     split. { tauto. }
-    intros. split. { apply (H2 _ H). }
+    intros. split. { apply H2. }
     tauto.
   - intros [z [H1 H2]].
     split. { tauto. }
-    intros. {apply (H2 _ H). }
+    intros. { apply H2,H. }
 Qed.
 
-Theorem Bin_Step_seq_sem_equiv:
-  Bin_Ter_seq_sem_equiv (BinRel.sem) (StepCnt.sem).
+Theorem Bin_Ter_seq_sem_equiv_true:
+  forall {T: Type} (mp: mid_param state T),
+  Bin_Ter_seq_sem_equiv (BinRel.sem) (TerSem.sem mp).
 Proof.
+  intros.
   unfold Bin_Ter_seq_sem_equiv. simpl.
   unfold Bin_Ter_sem_equiv. intros.
-  unfold BinRel.seq_sem, StepCnt.seq_sem, Relation_Operators.concat.
+  unfold BinRel.seq_sem, Relation_Operators.concat.
   split.
   - intros [st3 [H1 H2]].
     destruct (H st1 st3) as [H1' H1''].
     destruct (H1' H1) as [z1 HE1].
     destruct (H0 st3 st2) as [H2' H2''].
     destruct (H2' H2) as [z2 HE2].
-    exists (z1 + z2), z1, z2, st3.
+    exists (MP_add mp z1 z2), z1, z2, st3.
     tauto.
   - intros [z [z1 [z2 [st3 [H1 [H2 Hz]]]]]].
     destruct (H st1 st3) as [H1' H1''].
@@ -116,12 +122,14 @@ Proof.
       exists z2. apply H2.
 Qed.
 
-Theorem Bin_Step_if_sem_equiv:
-  Bin_Ter_if_sem_equiv (BinRel.sem) (StepCnt.sem).
+Theorem Bin_Ter_if_sem_equiv_true:
+  forall {T: Type} (mp: mid_param state T),
+  Bin_Ter_if_sem_equiv (BinRel.sem) (TerSem.sem mp).
 Proof.
+  intros.
   unfold Bin_Ter_if_sem_equiv. simpl.
   unfold Bin_Ter_sem_equiv. intros.
-  unfold semantic_if, BinRel.if_sem, StepCnt.if_sem.
+  unfold semantic_if, BinRel.if_sem, TerSem.if_sem.
   unfold Relation_Operators.union,
          Relation_Operators.concat,
          Relation_Operators.test_rel.
@@ -130,24 +138,21 @@ Proof.
     - destruct H1 as [st3 [[Hst Hb] H1]]. subst st3.
       destruct (H st1 st2) as [H' H''].
       destruct (H' H1) as [zc Hc].
-      exists (zc + 1). left.
-      exists 1, zc, st1.
+      exists (MP_add mp (MP_one mp st1 st1) zc). left.
+      exists (MP_one mp st1 st1), zc, st1.
       repeat split.
-      * unfold StepCnt.test_sem; tauto.
+      * tauto.
       * exact Hc.
-      * lia.
     - destruct H1 as [st3 [[Hst Hb] H1]]. subst st3.
       destruct (H0 st1 st2) as [H' H''].
       destruct (H' H1) as [zc Hc].
-      exists (zc + 1). right.
-      exists 1, zc, st1.
+      exists (MP_add mp (MP_one mp st1 st1) zc). right.
+      exists (MP_one mp st1 st1), zc, st1.
       repeat split.
-      * unfold StepCnt.test_sem; tauto.
+      * tauto.
       * exact Hc.
-      * lia.
   + destruct H1 as [z H1];
       destruct H1;
-      unfold StepCnt.seq_sem in H1;
       destruct H1 as [z1 [z2 [st3 [[Hst [Hb ?]] [Hc Hz]]]]];
       subst st3 z1 z.
     - destruct (H st1 st2) as [H' H''].
@@ -164,29 +169,30 @@ Proof.
         exists z2. exact Hc.
 Qed.
 
-Theorem Bin_Step_loop_sem_equiv:
-  Bin_Ter_loop_sem_equiv (BinRel.sem) (StepCnt.sem).
+Theorem Bin_Ter_loop_sem_equiv_true:
+  forall {T: Type} (mp: mid_param state T),
+  Bin_Ter_loop_sem_equiv (BinRel.sem) (TerSem.sem mp).
 Proof.
+  intros.
   unfold Bin_Ter_loop_sem_equiv. simpl.
   unfold Bin_Ter_sem_equiv. intros.
   unfold BinRel.loop_sem, Relation_Operators.omega_union.
-  unfold StepCnt.loop_sem, StepCnt.omega_union_sem.
   split; intros.
   + destruct H0 as [n H0].
     revert st1 st2 H0.
     induction n; intros; simpl in H0.
-    - exists 1, O. simpl.
+    - exists (MP_one mp st1 st2), O. simpl.
       unfold Relation_Operators.test_rel in H0.
-      unfold StepCnt.test_sem.
+      unfold TerSem.test_sem.
       tauto.
     - unfold Relation_Operators.concat, Relation_Operators.test_rel in H0.
       destruct H0 as [st1' [[Hst Hb] [st3 [H1 H2]]]]. subst st1'.
       destruct (IHn _ _ H2) as [zn [n_iter Hn]].
       destruct (H st1 st3) as [H' H''].
       destruct (H' H1) as [zc Hc].
-      exists (1 + (zc + zn)), (S n_iter).
-      simpl. unfold StepCnt.seq_sem.
-      exists 1, (zc + zn), st1.
+      exists (MP_add mp (MP_one mp st1 st1) (MP_add mp zc zn)), (S n_iter).
+      simpl. unfold TerSem.seq_sem.
+      exists (MP_one mp st1 st1), (MP_add mp zc zn), st1.
       repeat split.
       * exact Hb.
       * exists zc, zn, st3.
@@ -195,11 +201,10 @@ Proof.
     revert z st1 st2 H0.
     induction n; intros; simpl in H0.
     - exists O. simpl.
-      unfold StepCnt.test_sem in H0.
+      unfold TerSem.test_sem in H0.
       unfold Relation_Operators.test_rel.
       tauto.
-    - unfold StepCnt.seq_sem, StepCnt.test_sem in H0.
-      destruct H0 as [z0 [z1 [st1' [[Hst [Hb Ha0]] H0]]]].
+    - destruct H0 as [z0 [z1 [st1' [[Hst [Hb Ha0]] H0]]]].
       destruct H0 as [[zc [zn [st3 [Hz' [Hn' Hz2]]]]] Hz1].
       subst st1' z0 z1 z.
       destruct (IHn zn st3 st2 Hn') as [n_iter Hn].
@@ -209,151 +214,6 @@ Proof.
       exists st1. repeat split. { exact Hb. }
       exists st3. split.
       * apply H''. exists zc. exact Hz'.
-      * exact Hn.
-Qed.
-
-Theorem Bin_Trace_skip_sem_equiv:
-  Bin_Ter_skip_sem_equiv (BinRel.sem) (Trace.sem).
-Proof.
-  unfold Bin_Ter_skip_sem_equiv. simpl.
-  unfold Bin_Ter_sem_equiv. intros.
-  unfold BinRel.skip_sem, Trace.skip_sem.
-  split.
-  - intros. exists nil. tauto.
-  - intros [l [H1 H2]].
-    tauto.
-Qed.
-
-Theorem Bin_Trace_asgn_sem_equiv:
-  Bin_Ter_asgn_sem_equiv (BinRel.sem) (Trace.sem).
-Proof.
-  unfold Bin_Ter_asgn_sem_equiv. simpl.
-  unfold Bin_Ter_sem_equiv. intros.
-  unfold BinRel.asgn_sem, Trace.asgn_sem.
-  split.
-  - intros [H1 H2]. exists (st2 :: nil).
-    split. { tauto. }
-    intros. split. { apply (H2 _ H). }
-    tauto.
-  - intros [l [H1 H2]].
-    split. { tauto. }
-    intros. {apply (H2 _ H). }
-Qed.
-
-Theorem Bin_Trace_seq_sem_equiv:
-  Bin_Ter_seq_sem_equiv (BinRel.sem) (Trace.sem).
-Proof.
-  unfold Bin_Ter_seq_sem_equiv. simpl.
-  unfold Bin_Ter_sem_equiv. intros.
-  unfold BinRel.seq_sem, Trace.seq_sem, Relation_Operators.concat.
-  split.
-  - intros [st3 [H1 H2]].
-    destruct (H st1 st3) as [H1' H1''].
-    destruct (H1' H1) as [l1 HE1].
-    destruct (H0 st3 st2) as [H2' H2''].
-    destruct (H2' H2) as [l2 HE2].
-    exists (l1 ++ l2), l1, l2, st3.
-    tauto.
-  - intros [l [l1 [l2 [st3 [H1 [H2 Hl]]]]]].
-    destruct (H st1 st3) as [H1' H1''].
-    destruct (H0 st3 st2) as [H2' H2''].
-    exists st3.
-    split.
-    + apply H1''.
-      exists l1. apply H1.
-    + apply H2''.
-      exists l2. apply H2.
-Qed.
-
-Theorem Bin_Trace_if_sem_equiv:
-  Bin_Ter_if_sem_equiv (BinRel.sem) (Trace.sem).
-Proof.
-  unfold Bin_Ter_if_sem_equiv. simpl.
-  unfold Bin_Ter_sem_equiv. intros.
-  unfold semantic_if, BinRel.if_sem, Trace.if_sem.
-  unfold Relation_Operators.union,
-         Relation_Operators.concat,
-         Relation_Operators.test_rel.
-  split; intros.
-  + destruct H1.
-    - destruct H1 as [st3 [[Hst Hb] H1]]. subst st3.
-      destruct (H st1 st2) as [H' H''].
-      destruct (H' H1) as [lc Hc].
-      exists ((st1 :: nil) ++ lc). left.
-      exists (st1 :: nil), lc, st1.
-      repeat split.
-      * unfold Trace.test_sem; tauto.
-      * exact Hc.
-    - destruct H1 as [st3 [[Hst Hb] H1]]. subst st3.
-      destruct (H0 st1 st2) as [H' H''].
-      destruct (H' H1) as [lc Hc].
-      exists ((st1 :: nil) ++ lc). right.
-      exists (st1 :: nil), lc, st1.
-      repeat split.
-      * unfold Trace.test_sem; tauto.
-      * exact Hc.
-  + destruct H1 as [l H1];
-      destruct H1;
-      unfold Trace.seq_sem in H1;
-      destruct H1 as [l1 [l2 [st3 [[Hst [? Hb]] [Hc Hl]]]]];
-      subst st3 l1 l.
-    - destruct (H st1 st2) as [H' H''].
-      left. exists st1.
-      repeat split.
-      * exact Hb.
-      * apply H''. exists l2. exact Hc.
-    - destruct (H0 st1 st2) as [H' H''].
-      right. exists st1.
-      repeat split.
-      * exact Hb.
-      * apply H''. exists l2. exact Hc.
-Qed.
-
-Theorem Bin_Trace_loop_sem_equiv:
-  Bin_Ter_loop_sem_equiv (BinRel.sem) (Trace.sem).
-Proof.
-  unfold Bin_Ter_loop_sem_equiv. simpl.
-  unfold Bin_Ter_sem_equiv. intros.
-  unfold BinRel.loop_sem, Relation_Operators.omega_union.
-  unfold Trace.loop_sem, Trace.omega_union_sem.
-  split; intros.
-  + destruct H0 as [n H0].
-    revert st1 st2 H0.
-    induction n; intros; simpl in H0.
-    - exists (st1 :: nil), O. simpl.
-      unfold Relation_Operators.test_rel in H0.
-      unfold Trace.test_sem.
-      tauto.
-    - unfold Relation_Operators.concat, Relation_Operators.test_rel in H0.
-      destruct H0 as [st1' [[Hst Hb] [st3 [H1 H2]]]]. subst st1'.
-      destruct (IHn _ _ H2) as [ln [n_iter Hn]].
-      destruct (H st1 st3) as [H' H''].
-      destruct (H' H1) as [lc Hc].
-      exists ((st1 :: nil) ++ (lc ++ ln)), (S n_iter).
-      simpl. unfold Trace.seq_sem.
-      exists (st1 :: nil), (lc ++ ln), st1.
-      repeat split.
-      * exact Hb.
-      * exists lc, ln, st3.
-        repeat split; [exact Hc | exact Hn].
-  + destruct H0 as [l [n H0]].
-    revert l st1 st2 H0.
-    induction n; intros; simpl in H0.
-    - exists O. simpl.
-      unfold Trace.test_sem in H0.
-      unfold Relation_Operators.test_rel.
-      tauto.
-    - unfold Trace.seq_sem, Trace.test_sem in H0.
-      destruct H0 as [l0 [l1 [st1' [[Hst [Ha0 Hb]] H0]]]].
-      destruct H0 as [[lc [ln [st3 [Hl' [Hn' Hl2]]]]] Hl1].
-      subst st1' l0 l1 l.
-      destruct (IHn ln st3 st2 Hn') as [n_iter Hn].
-      destruct (H st1 st3) as [H' H''].
-      exists (S n_iter). simpl.
-      unfold Relation_Operators.concat, Relation_Operators.test_rel.
-      exists st1. repeat split. { exact Hb. }
-      exists st3. split.
-      * apply H''. exists lc. exact Hl'.
       * exact Hn.
 Qed.
 
@@ -390,19 +250,23 @@ Qed.
 Theorem Bin_Step_equiv:
   sem_equiv (BinRel.ceval) (StepCnt.ceval) (Bin_Ter_sem_equiv).
 Proof.
-  apply (command_equiv__sem_equiv Z BinRel.sem StepCnt.sem
-    Bin_Step_skip_sem_equiv Bin_Step_asgn_sem_equiv
-    Bin_Step_seq_sem_equiv  Bin_Step_if_sem_equiv
-    Bin_Step_loop_sem_equiv).
+  apply (command_equiv__sem_equiv _ _ _
+    (Bin_Ter_skip_sem_equiv_true _)
+    (Bin_Ter_asgn_sem_equiv_true _)
+    (Bin_Ter_seq_sem_equiv_true  _)
+    (Bin_Ter_if_sem_equiv_true   _)
+    (Bin_Ter_loop_sem_equiv_true _)).
 Qed.
 
 Theorem Bin_Trace_equiv:
   sem_equiv (BinRel.ceval) (Trace.ceval) (Bin_Ter_sem_equiv).
 Proof.
-  apply (command_equiv__sem_equiv (list state) BinRel.sem Trace.sem
-    Bin_Trace_skip_sem_equiv Bin_Trace_asgn_sem_equiv
-    Bin_Trace_seq_sem_equiv  Bin_Trace_if_sem_equiv
-    Bin_Trace_loop_sem_equiv).
+  apply (command_equiv__sem_equiv _ _ _
+    (Bin_Ter_skip_sem_equiv_true _)
+    (Bin_Ter_asgn_sem_equiv_true _)
+    (Bin_Ter_seq_sem_equiv_true  _)
+    (Bin_Ter_if_sem_equiv_true   _)
+    (Bin_Ter_loop_sem_equiv_true _)).
 Qed.
 
 (* General Theorem for equivalence between two recursively defined semantics *)
