SmallStepSemEquiv.v
@@ -4,10 +4,17 @@ Require Import PL.ImpExt4.
 Require Import PL.DenotationalSemantics.
 Require Import PL.SmallStepSemantics.
 
-(* General Theorem for equivalence between a denotational semantics and small step semantics. *)
+(** General Theorem for equivalence between a denotational semantics and small step semantics.
+    The theorem for the equivalence between a denotational semantics and small step semantics is proven in 2 cases: one for binary denotational semantics, another for ternary denotational semantics *)
+
+(** The overall proof idea is almost the same as taught in class:
+    1. Denotation --> Small step:
+        By induction and congruence rules.
+    2. Small step --> Denotation:
+        By proving that taking a small step preserve the result. *)
 
 (* ################################################################# *)
-(** * Congruence Theorems of Multi-step Relations *)
+(* Basic Congruence Theorems of Multi-step Relations *)
 
 Theorem multi_congr_APlus1: forall st a1 a1' a2,
   multi_astep st a1 a1' ->
@@ -351,8 +358,15 @@ Proof.
 Qed.
 
 (** Lemmas Finished *)
+
+(* ################################################################# *)
+(* Equivalence Between Binary Denotational Semantics & Small Step Semantics *)
+
 Local Open Scope imp.
 
+Module BinEquiv.
+
+(** Any step in simplifying aexp corresponds to a step in simplifying cexp. *)
 Theorem multi_congr_CAss: forall st X a a',
   multi_astep st a a' ->
   BinStep.multi_cstep (CAss X a, st) (CAss X a', st).
@@ -366,6 +380,7 @@ Proof.
       exact H.
 Qed.
 
+(** A step in a single cexp corresponds to a step in a sequence of cexp, which execute the same cexp at first. *)
 Theorem multi_congr_CSeq: forall st1 c1 st1' c1' c2,
   BinStep.multi_cstep (c1, st1) (c1', st1') ->
   BinStep.multi_cstep (CSeq c1 c2, st1) (CSeq c1' c2, st1').
@@ -379,6 +394,7 @@ Proof.
       exact H.
 Qed.
 
+(** Any step in simplifying bexp corresponds to a step in simplifying cexp. *)
 Theorem multi_congr_CIf: forall st b b' c1 c2,
   multi_bstep st b b' ->
   BinStep.multi_cstep
@@ -423,33 +439,24 @@ Proof.
     apply IHn, H2.
 Qed.
 
+(** First direction: Denotation --> Small Step *)
 Theorem semantic_equiv_com1: forall st1 st2 c,
   BinRel.ceval c st1 st2 -> BinStep.multi_cstep (c, st1) (Skip, st2).
 Proof.
   intros.
-  revert st1 st2 H; induction c; intros.
-  + rewrite BinRel.ceval_CSkip in H.
-    unfold Relation_Operators.id in H.
-    rewrite H.
+  revert st1 st2 H; induction c; simpl; intros; unfold BinRel.ceval,BinRel.sem,ceval_by_sem in H; simpl in H.
+  + rewrite H.
     reflexivity.
-  + rewrite BinRel.ceval_CAss in H.
-    destruct H.
+  + destruct H.
     BinStep.etransitivity_n1.
     - apply multi_congr_CAss, semantic_equiv_aexp1.
       reflexivity.
     - apply BinStep.CS_Ass; tauto.
-  + rewrite BinRel.ceval_CSeq in H.
-    unfold Relation_Operators.concat in H.
-    destruct H as [st' [? ?]].
+  + destruct H as [st' [? ?]].
     etransitivity; [apply multi_congr_CSeq, IHc1, H |].
     BinStep.etransitivity_1n; [ apply BinStep.CS_Seq |].
     apply IHc2, H0.
-  + rewrite BinRel.ceval_CIf in H.
-    unfold if_sem in H.
-    unfold Relation_Operators.union,
-           Relation_Operators.concat,
-           Relation_Operators.test_rel in H.
-    pose proof semantic_equiv_bexp1 st1 b.
+  + pose proof semantic_equiv_bexp1 st1 b.
     destruct H0.
     destruct H as [H | H]; destruct H as [st [[? ?] ?]]; subst st.
     - etransitivity; [apply multi_congr_CIf, H0, H2 |].
@@ -458,17 +465,13 @@ Proof.
     - etransitivity; [apply multi_congr_CIf, H1, H2 |].
       BinStep.etransitivity_1n; [apply BinStep.CS_IfFalse |].
       apply IHc2, H3.
-  + rewrite BinRel.ceval_CWhile in H.
-    unfold loop_sem in H.
-    unfold Relation_Operators.omega_union in H.
-    destruct H as [n ?].
+  + destruct H as [n ?].
     apply semantic_equiv_iter_loop1 with n.
     - exact IHc.
     - exact H.
 Qed.
 
-Print ceval_CAss.
-
+(** Any small step from a pair (c1, st1) to (c2, st2) will not change the result of its denotation. *)
 Lemma ceval_preserve: forall c1 c2 st1 st2,
   BinStep.cstep (c1, st1) (c2, st2) ->
   forall st3, BinRel.ceval c2 st2 st3 -> BinRel.ceval c1 st1 st3.
@@ -480,30 +483,28 @@ Proof.
   revert H0.
   remember (c1, st1) as cst1 eqn:H0.
   remember (c2, st2) as cst2 eqn:H1.
-  revert c1 c2 st1 st2 st3 H0 H1; induction H; simpl; intros.
+  revert c1 c2 st1 st2 st3 H0 H1; unfold BinRel.ceval,BinRel.sem,ceval_by_sem; induction H; subst; simpl; intros.
   + apply aeval_preserve in H.
     injection H0 as ? ?.
     injection H1 as ? ?.
     subst.
-    rewrite BinRel.ceval_CAss in H2.
-    rewrite BinRel.ceval_CAss.
+    simpl.
+    unfold BinRel.asgn_sem.
     rewrite H.
     tauto.
   + injection H1 as ? ?.
     injection H2 as ? ?.
     subst.
-    rewrite BinRel.ceval_CSkip in H3.
-    rewrite BinRel.ceval_CAss.
-    unfold Relation_Operators.id in H3.
+    simpl. simpl in H3.
+    unfold BinRel.skip_sem,Relation_Operators.id in H3.
+    unfold BinRel.asgn_sem.
     subst.
     tauto.
   + injection H0 as ? ?.
     injection H1 as ? ?.
     subst.
-    rewrite BinRel.ceval_CSeq in H2.
-    rewrite BinRel.ceval_CSeq.
-    unfold Relation_Operators.concat in H2.
-    unfold Relation_Operators.concat.
+    unfold BinRel.seq_sem,Relation_Operators.concat in H2.
+    unfold BinRel.seq_sem,Relation_Operators.concat.
     destruct H2 as [st2' [? ?]].
     exists st2'.
     assert ((c1, st1) = (c1, st1)). { reflexivity. }
@@ -520,8 +521,6 @@ Proof.
   + injection H0 as ? ?.
     injection H1 as ? ?.
     subst.
-    rewrite BinRel.ceval_CIf in H2.
-    rewrite BinRel.ceval_CIf.
     unfold BinRel.if_sem in H2.
     unfold BinRel.if_sem.
     unfold Relation_Operators.union,
@@ -540,7 +539,6 @@ Proof.
   + injection H0 as ? ?.
     injection H1 as ? ?.
     subst.
-    rewrite BinRel.ceval_CIf.
     unfold BinRel.if_sem.
     unfold Relation_Operators.union,
            Relation_Operators.concat,
@@ -550,7 +548,6 @@ Proof.
   + injection H0 as ? ?.
     injection H1 as ? ?.
     subst.
-    rewrite BinRel.ceval_CIf.
     unfold BinRel.if_sem.
     unfold Relation_Operators.union,
            Relation_Operators.concat,
@@ -565,6 +562,7 @@ Proof.
     tauto.
 Qed.
 
+(** Second direction: Small Step --> Denotation *)
 Theorem semantic_equiv_com2: forall c st1 st2,
   BinStep.multi_cstep (c, st1) (CSkip, st2) -> BinRel.ceval c st1 st2.
 Proof.
@@ -576,6 +574,8 @@ Proof.
     tauto.
 Qed.
 
+(* ################################################################# *)
+(* Final theorem for binary denotational semantics *)
 Theorem semantic_equiv: forall c st1 st2,
   BinRel.ceval c st1 st2 <-> BinStep.multi_cstep (c, st1) (CSkip, st2).
 Proof.
@@ -584,3 +584,275 @@ Proof.
   + apply semantic_equiv_com1.
   + apply semantic_equiv_com2.
 Qed.
+
+End BinEquiv.
+
+(* ################################################################# *)
+(* Equivalence between ternary denotational semantics & small step semantics *)
+
+(** In the proof, we used a concept “Middle parameter” to denote the step count (or trace) in the corresponding denotational semantics. *)
+
+Module TerEquiv.
+
+Theorem multi_congr_CAss: forall B (mp : mid_param state B) st X a a',
+  multi_astep st a a' ->
+  TerStep.multi_cstep mp
+  (CAss X a, st) (MP_zero mp) (CAss X a', st).
+Proof.
+  intros.
+  induction_n1 H.
+  + destruct mp. TerStep.rt_reflexivity.
+  + TerStep.etransitivity_n1.
+    - exact IHrt.
+    - instantiate (b:=false). reflexivity.
+    - apply TerStep.CS_AssStep.
+      exact H.
+Qed.
+
+Theorem multi_congr_CIf: forall B (mp : mid_param state B) st b b' c1 c2,
+  multi_bstep st b b' ->
+  TerStep.multi_cstep mp
+    (CIf b c1 c2, st)
+    (MP_zero mp)
+    (CIf b' c1 c2, st).
+Proof.
+  intros.
+  induction_n1 H.
+  + destruct mp. TerStep.rt_reflexivity.
+  + TerStep.etransitivity_n1.
+    - exact IHrt.
+    - instantiate (b0:=false). reflexivity.
+    - apply TerStep.CS_IfStep.
+      exact H.
+Qed.
+
+Theorem multi_congr_CSeq: forall B (mp : mid_param state B) st1 c1 st1' c1' c2 cnt,
+  TerStep.multi_cstep mp (c1, st1) cnt (c1', st1') ->
+  TerStep.multi_cstep mp (CSeq c1 c2, st1) cnt (CSeq c1' c2, st1').
+Proof.
+  intros.
+  TerStep.induction_n1 H.
+  + TerStep.rt_reflexivity.
+  + TerStep.etransitivity_n1.
+    - exact IHrt.
+    - instantiate (b:=false). reflexivity.
+    - apply TerStep.CS_SeqStep.
+      exact H.
+  + TerStep.etransitivity_n1.
+    - exact IHrt.
+    - instantiate (b:=true). subst.
+      destruct mp. reflexivity.
+    - apply TerStep.CS_SeqStep.
+      exact H.
+Qed.
+
+Lemma semantic_equiv_iter_loop1: forall B (mp : mid_param state B) st1 st2 n b c cnt,
+  (forall st1 cnt st2, TerSem.ceval mp c st1 cnt st2 -> TerStep.multi_cstep mp (c, st1) cnt (CSkip, st2)) ->
+  TerSem.iter_loop_body mp b (TerSem.ceval mp c) n st1 cnt st2 ->
+  TerStep.multi_cstep mp (While b Do c EndWhile, st1) cnt (CSkip, st2).
+Proof.
+  intros.
+  destruct mp; revert st1 st2 cnt H0; induction n; simpl; intros.
+  + simpl in H0.
+    destruct H0.
+    subst st2.
+    TerStep.etransitivity_1n ; [apply TerStep.CS_While | reflexivity |].
+    TerStep.rt_etransitivity; [apply multi_congr_CIf, semantic_equiv_bexp1_false, H1 | simpl; rewrite add_zero_l; reflexivity |].
+    TerStep.etransitivity_1n; [apply TerStep.CS_IfFalse | |].
+    { destruct H1. subst cnt. instantiate (c':=zero). simpl. rewrite add_zero_r. reflexivity. }
+    TerStep.rt_reflexivity.
+  + simpl in H0.
+    unfold TerSem.seq_sem at 1,
+           TerSem.test_sem in H0.
+    destruct H0 as [t1 [t2 [st [[? [H0 ?]] [? ?]]]]]; subst st.
+    destruct H3 as [t1' [t2' [st1' [? [? ?]]]]].
+    TerStep.etransitivity_1n; [apply TerStep.CS_While | reflexivity |].
+    TerStep.rt_etransitivity; [apply multi_congr_CIf, semantic_equiv_bexp1_true, H0 | simpl; rewrite add_zero_l; reflexivity |].
+    TerStep.etransitivity_1n; [apply TerStep.CS_IfTrue | subst; reflexivity |].
+    TerStep.rt_etransitivity; [apply multi_congr_CSeq,H,H1 | subst; reflexivity |].
+    TerStep.etransitivity_1n; [apply TerStep.CS_Seq | reflexivity |].
+    apply IHn, H3.
+Qed.
+
+Theorem semantic_equiv_com1: forall B (mp : mid_param state B) st1 st2 c cnt,
+  TerSem.ceval mp c st1 cnt st2 -> TerStep.multi_cstep mp (c, st1) cnt (Skip, st2).
+Proof.
+  intros.
+  destruct mp; revert st1 cnt st2 H; induction c; simpl; unfold TerSem.ceval,TerStep.extend_mp; simpl; intros.
+  + destruct H; subst.
+    TerStep.rt_reflexivity.
+  + destruct H as [? [? ?]].
+    TerStep.etransitivity_n1.
+    - apply multi_congr_CAss, semantic_equiv_aexp1.
+      reflexivity.
+    - instantiate (1:=true). simpl. rewrite add_zero_l. apply H1.
+    - apply TerStep.CS_Ass; tauto.
+  + destruct H as [t1 [t2 [st' [? [? ?]]]]].
+    TerStep.rt_etransitivity; [apply multi_congr_CSeq, IHc1, H | apply H1 |].
+    TerStep.etransitivity_1n; [ apply TerStep.CS_Seq | reflexivity |].
+    apply IHc2, H0.
+  + pose proof semantic_equiv_bexp1 st1 b.
+    destruct H0.
+    destruct H as [H | H]; destruct H as [t1 [t2 [st [[? [? ?]] [? ?]]]]]; subst st.
+    - TerStep.rt_etransitivity; [apply multi_congr_CIf, H0, H2 | simpl; rewrite add_zero_l; reflexivity |].
+      TerStep.etransitivity_1n; [apply TerStep.CS_IfTrue | subst; reflexivity |].
+      subst. apply IHc1, H4.
+    - TerStep.rt_etransitivity; [apply multi_congr_CIf, H1, H2 | simpl; rewrite add_zero_l; reflexivity |].
+      TerStep.etransitivity_1n; [apply TerStep.CS_IfFalse | subst; reflexivity |].
+      subst. apply IHc2, H4.
+  + destruct H as [n ?].
+    apply semantic_equiv_iter_loop1 with n.
+    - exact IHc.
+    - exact H.
+Qed.
+
+(** Need 2 lemmas in 2 cases: one lemma for the small step that does not change  step count (or trace), another lemma for the small step that changes step count (or trace). *)
+Lemma ceval_preserve_false: forall B (mp : mid_param state B) c1 c2 st1 st2 cnt,
+  TerStep.cstep (c1, st1) false (c2, st2) ->
+  forall st3, TerSem.ceval mp c2 st2 cnt st3 -> TerSem.ceval mp c1 st1 cnt st3.
+Proof.
+  intros.
+  revert H0.
+  remember (c1, st1) as cst1 eqn:H0.
+  remember (c2, st2) as cst2 eqn:H1.
+  remember false as b eqn:Hb.
+  revert c1 c2 st1 st2 st3 cnt H0 H1. unfold TerSem.ceval; induction H; subst; intros; destruct mp eqn:Emp.
+  + apply aeval_preserve in H.
+    injection H0 as ? ?.
+    injection H1 as ? ?.
+    subst. simpl. simpl in H2.
+    unfold TerSem.asgn_sem.
+    rewrite H.
+    tauto.
+  + inversion Hb.
+  + injection H0 as ? ?.
+    injection H1 as ? ?.
+    subst.
+    rewrite ceval_CSeq in H2.
+    rewrite ceval_CSeq.
+    simpl in H2. unfold TerSem.seq_sem in H2.
+    simpl. unfold TerSem.seq_sem.
+    destruct H2 as [t1 [t2 [st2' [? [? ?]]]]].
+    exists t1,t2,st2'.
+    pose proof (IHcstep eq_refl _ _ _ _ _ _ eq_refl eq_refl H0).
+    tauto.
+  + injection H0 as ? ?.
+    injection H1 as ? ?.
+    subst.
+    exists zero,cnt,st2.
+    split.
+    - rewrite ceval_CSkip. simpl.
+      unfold TerSem.skip_sem. tauto.
+    - split; [exact H2 | simpl; rewrite add_zero_l; reflexivity].
+  + injection H0 as ? ?.
+    injection H1 as ? ?.
+    subst.
+    rewrite ceval_CIf in H2.
+    rewrite ceval_CIf.
+    simpl in H2. simpl.
+    unfold TerSem.if_sem,TerSem.union_sem,TerSem.seq_sem,TerSem.test_sem in H2.
+    unfold TerSem.if_sem,TerSem.union_sem,TerSem.seq_sem,TerSem.test_sem.
+    apply beval_preserve in H.
+    simpl in H2.
+    simpl.
+    unfold Sets.complement in H2.
+    unfold Sets.complement.
+    destruct H2 as [[t1 [t2 [st2' ?]]] | [t1 [t2 [st2' ?]]]]; [left | right];
+      exists t1,t2,st2'; tauto.
+  + inversion Hb.
+  + inversion Hb.
+  + injection H0 as ? ?.
+    injection H1 as ? ?.
+    pose proof TerSem.loop_unrolling mp b c.
+    subst.
+    specialize (H4 cnt st2 st3).
+    tauto.
+Qed.
+
+Lemma ceval_preserve_true: forall B (mp : mid_param state B) c1 c2 st1 st2 cnt,
+  TerStep.cstep (c1, st1) true (c2, st2) ->
+  forall st3, TerSem.ceval mp c2 st2 cnt st3 -> TerSem.ceval mp c1 st1 (MP_add mp (MP_one mp st1 st2) cnt) st3.
+Proof.
+  intros.
+  revert H0.
+  remember (c1, st1) as cst1 eqn:H0.
+  remember (c2, st2) as cst2 eqn:H1.
+  remember true as b eqn:Hb.
+  revert c1 c2 st1 st2 st3 cnt H0 H1. unfold TerSem.ceval; induction H; intros.
+  + inversion Hb.
+  + injection H1 as ? ?.
+    injection H2 as ? ?.
+    subst.
+    simpl. simpl in H3.
+    unfold TerSem.skip_sem in H3.
+    unfold TerSem.asgn_sem.
+    destruct H3. subst.
+    split. tauto. split. tauto. simpl. rewrite (MP_add_zero_r mp). reflexivity.
+  + injection H0 as ? ?.
+    injection H1 as ? ?.
+    subst. destruct mp.
+    simpl. simpl in H2.
+    unfold TerSem.seq_sem in H2.
+    unfold TerSem.seq_sem.
+    destruct H2 as [t1 [t2 [st2' [? [? ?]]]]].
+    pose proof (IHcstep eq_refl _ _ _ _ _ _ eq_refl eq_refl H0).
+    exists (add (one st1 st2) t1),t2,st2'.
+    subst. simpl. split; [tauto|split; [tauto|]]. rewrite <- add_assoc.
+    tauto.
+  + inversion Hb.
+  + inversion Hb.
+  + injection H0 as ? ?.
+    injection H1 as ? ?.
+    subst. destruct mp.
+    left; exists (one st2 st2),cnt,st2; simpl.
+    unfold Sets.full,TerSem.test_sem. tauto.
+  + injection H0 as ? ?.
+    injection H1 as ? ?.
+    subst. destruct mp.
+    right; exists (one st2 st2),cnt,st2; simpl.
+    unfold TerSem.test_sem,Sets.complement, Sets.empty. tauto.
+  + inversion Hb.
+Qed.
+
+Theorem semantic_equiv_com2: forall B (mp : mid_param state B) c st1 st2 cnt,
+  TerStep.multi_cstep mp (c, st1) cnt (CSkip, st2) -> TerSem.ceval mp c st1 cnt st2.
+Proof.
+  intros.
+  remember (CSkip) as c' eqn:H0.
+  revert H0; TerStep.induction_1n H; simpl; intros; subst.
+  + unfold TerSem.ceval. simpl. destruct mp. unfold TerSem.skip_sem. tauto.
+  + specialize (IHrt eq_refl).
+    pose proof ceval_preserve_false _ mp _ _ _ _ _ H st2 IHrt.
+    tauto.
+  + specialize (IHrt eq_refl).
+    pose proof ceval_preserve_true _ mp _ _ _ _ _ H st2 IHrt.
+    destruct mp.
+    tauto.
+Qed.
+
+Theorem semantic_equiv: forall B (mp : mid_param state B) c st1 cnt st2,
+  TerSem.ceval mp c st1 cnt st2 <-> TerStep.multi_cstep mp (c, st1) cnt (CSkip, st2).
+Proof.
+  intros.
+  split.
+  + apply semantic_equiv_com1.
+  + apply semantic_equiv_com2.
+Qed.
+
+(* ################################################################# *)
+(* Final theorem for ternary denotational semantics *)
+
+Theorem semantic_equiv_StepCnt: forall c st1 cnt st2,
+  StepCnt.ceval c st1 cnt st2 <-> TerStep.multi_cstep_cnt (c, st1) cnt (CSkip, st2).
+Proof.
+  apply semantic_equiv.
+Qed.
+
+Theorem semantic_equiv_Trace: forall c st1 l st2,
+  Trace.ceval c st1 l st2 <-> TerStep.multi_cstep_trace (c, st1) l (CSkip, st2).
+Proof.
+  apply semantic_equiv.
+Qed.
+
+End TerEquiv.
+
